SetPartition.supp sSup is not longer in the type

Kura/Dep/SetPartition.lean
@@ -1,9 +1,9 @@
 import Mathlib.Data.Setoid.Partition
 import Mathlib.Data.SetLike.Basic
 import Mathlib.Data.Set.Finite.Powerset
-import Matroid.ForMathlib.SetPartition
+-- import Matroid.ForMathlib.Lattice
 
-open Set Partition
+open Set
 
 variable {α : Type*} {s x y z : α}
 
@@ -11,13 +11,628 @@ variable {α : Type*} {s x y z : α}
 lemma Set.ext_iff_simp {α : Type*} {P Q : α → Prop} : {x | P x} = {x | Q x} ↔ ∀ x, P x ↔ Q x :=
   Set.ext_iff
 
+structure Partition (α : Type*) [CompleteLattice α] where
+  parts : Set α
+  indep : sSupIndep parts
+  bot_not_mem : ⊥ ∉ parts
+
+namespace Partition
+
+section Basic
+
+variable [CompleteLattice α] {P : Partition α}
+
+def supp (P : Partition α) : α := sSup P.parts
+
+instance {α : Type*} [CompleteLattice α] : SetLike (Partition α) α where
+  coe := Partition.parts
+  coe_injective' p p' h := by cases p; cases p'; simpa using h
+
+@[simp] lemma mem_parts {x : α} : x ∈ P.parts ↔ x ∈ (P : Set α) := Iff.rfl
+
+@[ext] lemma ext {P Q : Partition α} (hP : ∀ x, x ∈ P ↔ x ∈ Q) : P = Q := by
+  cases P
+  cases Q
+  simp only [mk.injEq]
+  ext x
+  simpa using hP x
+
+lemma disjoint (hx : x ∈ P) (hy : y ∈ P) (hxy : x ≠ y) :
+    Disjoint x y :=
+  P.indep.pairwiseDisjoint hx hy hxy
+
+lemma pairwiseDisjoint : Set.PairwiseDisjoint (P : Set α) id :=
+  fun _ hx _ hy hxy ↦ P.disjoint hx hy hxy
+
+lemma ne_bot_of_mem (hx : x ∈ P) : x ≠ ⊥ :=
+  fun h ↦ P.bot_not_mem <| h ▸ hx
+
+lemma bot_lt_of_mem (hx : x ∈ P) : ⊥ < x :=
+  bot_lt_iff_ne_bot.2 <| P.ne_bot_of_mem hx
+
+lemma sSup_eq (P : Partition α) : sSup P = P.supp  := rfl
+
+lemma iSup_eq (P : Partition α) : ⨆ x ∈ P, x = P.supp := by
+  simp_rw [← P.sSup_eq, sSup_eq_iSup]
+  rfl
+
+lemma le_of_mem (P : Partition α) (hx : x ∈ P) : x ≤ P.supp :=
+  (le_sSup hx).trans_eq P.sSup_eq
+
+lemma parts_nonempty (P : Partition α) (hs : P.supp ≠ ⊥) : (P : Set α).Nonempty :=
+  nonempty_iff_ne_empty.2 fun hP ↦ by simp [← P.sSup_eq, hP, sSup_empty] at hs
+
+-- @[simps] protected def congr {t : α} (P : Partition s) (hst : s = t) : Partition t where
+--   parts := P.parts
+--   indep := P.indep
+--   bot_not_mem := P.bot_not_mem
+--   sSup_eq' := hst ▸ P.sSup_eq'
+
+-- @[simp] lemma coe_congr_eq {t : α} {P : Partition s} (hst : s = t) :
+--     (P.congr hst : Set α) = P := rfl
+
+-- @[simp] lemma mem_congr_iff {t x : α} {P : Partition s} (hst : s = t) :
+--     x ∈ P.congr hst ↔ x ∈ P := Iff.rfl
+
+-- @[simps!] def partsCongrEquiv {t : α} (P : Partition s) (hst : s = t) :
+--     (P : Set α) ≃ (P.congr hst : Set α) := Equiv.setCongr rfl
+
+end Basic
+
+section indep
+
+variable [CompleteLattice α]
+
+/-- A `sSupIndep` collection not containing `⊥` gives a partition of its supremum. -/
+@[simps] def ofIndependent {u : Set α} (hs : sSupIndep u) (hbot : ⊥ ∉ u) : Partition α where
+  parts := u
+  indep := hs
+  bot_not_mem := hbot
+
+@[simp] lemma mem_ofIndependent_iff {u : Set α} (hu : sSupIndep u)
+    (h : ⊥ ∉ u) {a : α} : a ∈ ofIndependent hu h ↔ a ∈ u := Iff.rfl
+
+@[simp] lemma supp_ofIndependent {u : Set α} (hu : sSupIndep u) (hbot : ⊥ ∉ u) :
+    (ofIndependent hu hbot).supp = sSup u := rfl
+
+/-- A `sSupIndep` collection gives a partition of its supremum by removing `⊥`. -/
+def ofIndependent' {u : Set α} (hs : sSupIndep u) : Partition α :=
+  (ofIndependent (hs.mono (diff_subset (t := {⊥}))) (fun h ↦ h.2 rfl))
+
+@[simp] lemma mem_ofIndependent'_iff {u : Set α} (hu : sSupIndep u) {a : α} :
+  a ∈ ofIndependent' hu ↔ a ∈ u ∧ a ≠ ⊥ := Iff.rfl
+
+@[simp] lemma supp_ofIndependent' {u : Set α} (hu : sSupIndep u) :
+    (ofIndependent' hu).supp = sSup u := by
+  show sSup (u \ {⊥}) = sSup u
+  simp
+
+/-- The partition with no parts. -/
+@[simps] protected def empty (α : Type*) [CompleteLattice α] : Partition α where
+  parts := ∅
+  indep := by simp
+  bot_not_mem := by simp
+
+@[simp] lemma empty_coe_eq (α : Type*) [CompleteLattice α] :
+    (Partition.empty α : Set α) = ∅ := rfl
+
+@[simp] lemma not_mem_empty (α : Type*) [CompleteLattice α] {a : α} :
+    a ∉ Partition.empty α := by
+  rw [← SetLike.mem_coe, empty_coe_eq]
+  simp
+
+@[simp] lemma supp_empty (α : Type*) [CompleteLattice α] : (Partition.empty α).supp = ⊥ := by
+  simp [Partition.empty, supp]
+
+lemma eq_empty {P : Partition α} (hP : P.supp = ⊥) : P = Partition.empty α := by
+  ext x
+  have hsup := P.sSup_eq
+  simp only [sSup_eq_bot, SetLike.mem_coe, hP] at hsup
+  simp only [not_mem_empty, iff_false]
+  exact fun hx ↦ P.ne_bot_of_mem hx <| hsup x hx
+
+instance {α : Type*} [CompleteLattice α] [Subsingleton α] : Unique (Partition α) where
+  default := Partition.empty α
+  uniq P := eq_empty (by
+    simp only [← P.sSup_eq, sSup_eq_bot, SetLike.mem_coe]
+    exact fun a b ↦ Subsingleton.elim _ _)
+
+/-- The one-part partition. -/
+@[simps] def indiscrete (s : α) (hs : s ≠ ⊥) : Partition α where
+  parts := {s}
+  indep := by simp [sSupIndep]
+  bot_not_mem := by simpa using hs.symm
+
+@[simp] lemma mem_indiscrete_iff (s : α) (hs : s ≠ ⊥) {a : α} :
+    a ∈ Partition.indiscrete s hs ↔ a = s := Iff.rfl
+
+lemma supp_indiscrete (s : α) (hs : s ≠ ⊥) : (Partition.indiscrete s hs).supp = s := by
+  simp [Partition.indiscrete, supp]
+
+end indep
+
+section Order
+
+variable {α : Type*} [CompleteLattice α] {s : α}
+
+instance : PartialOrder (Partition α) where
+  le P Q := ∀ x ∈ P, ∃ y ∈ Q, x ≤ y
+  lt := _
+  le_refl P x hx := by
+    refine ⟨x,hx,rfl.le⟩
+  le_trans P Q R hPQ hQR x hxP := by
+    obtain ⟨y, hy, hxy⟩ := hPQ x hxP
+    obtain ⟨z, hz, hyz⟩ := hQR y hy
+    exact ⟨z, hz, hxy.trans hyz⟩
+  le_antisymm P Q hp hq := by
+    refine Partition.ext fun x ↦ ⟨fun h ↦ ?_, fun h ↦ ?_⟩
+    · obtain ⟨y, hy, hxy⟩ := hp x h
+      obtain ⟨x', hx', hyx'⟩ := hq y hy
+      obtain rfl := PairwiseDisjoint.eq_of_le P.pairwiseDisjoint h hx' (P.ne_bot_of_mem h)
+        (hxy.trans hyx')
+      rwa [hxy.antisymm hyx']
+    obtain ⟨y, hy, hxy⟩ := hq x h
+    obtain ⟨x', hx', hyx'⟩ := hp y hy
+    obtain rfl := PairwiseDisjoint.eq_of_le Q.pairwiseDisjoint h hx' (Q.ne_bot_of_mem h)
+      (hxy.trans hyx')
+    rwa [hxy.antisymm hyx']
+
+instance : OrderTop (Partition α) where
+  top := ofIndependent' (sSupIndep_singleton ⊤)
+  le_top := by
+    obtain (hs | hs) := eq_or_ne ⊤ (⊥ : α)
+    · have : Subsingleton α := subsingleton_of_bot_eq_top hs.symm
+      simp [hs]
+    exact fun P x hx ↦ ⟨⊤, by simp [hs], by simp⟩
+
+@[simp] lemma mem_top_iff {a : α} : a ∈ (⊤ : Partition α) ↔ a = ⊤ ∧ a ≠ ⊥ := by
+  change a ∈ ofIndependent' (sSupIndep_singleton ⊤) ↔ _
+  rw [mem_ofIndependent'_iff, mem_singleton_iff]
+
+lemma top_eq_indiscrete (hs : ⊤ ≠ ⊥) : (⊤ : Partition α) = indiscrete ⊤ hs := by
+  ext a
+  rw [mem_top_iff, mem_indiscrete_iff, and_iff_left_iff_imp]
+  rintro rfl; assumption
+
+lemma parts_top_subset : ((⊤ : Partition α) : Set α) ⊆ {⊤} := by
+  simp
+
+
+end Order
+section Bind
+
+variable {α : Type*} [CompleteDistribLattice α]
+
+-- @[simps] protected def bind (P : Partition α) (Qs : ∀ a ∈ P, Partition α)
+--     (hQs : ∀ a, (h : a ∈ P) → (Qs a h).supp = a) : Partition α where
+--   parts := ⋃ a : P, (Qs a a.prop)
+--   indep b hb := by
+--     simp only [mem_iUnion, SetLike.mem_coe, Subtype.exists] at hb
+--     obtain ⟨a, haP, hba : b ∈ Qs a haP⟩ := hb
+--     have hdj1 := (Qs a haP).indep hba
+--     have hdj2 := (P.indep haP).mono_left <| (Qs a haP).le_of_mem hba
+--     refine (hdj1.sup_right hdj2).mono_right ?_
+--     simp only [mem_iUnion, SetLike.mem_coe, Subtype.exists, not_exists, mem_parts, ge_iff_le,
+--       sSup_le_iff, mem_diff, mem_singleton_iff, and_imp, forall_exists_index]
+
+--     rintro t' x hx (ht' : t' ∈ Qs x hx) hne
+--     obtain (rfl | hne) := eq_or_ne x a
+--     · exact (le_sSup_of_le (show t' ∈ _ \ {b} from ⟨ht', hne⟩) rfl.le).trans le_sup_left
+--     exact (le_sSup_of_le (show x ∈ P.parts \ ({a} : Set α) from ⟨hx, hne⟩)
+--       ((Qs x hx).le_of_mem ht')).trans le_sup_right
+--   bot_not_mem := by
+--     simp only [mem_iUnion, SetLike.mem_coe, Subtype.exists, not_exists]
+--     exact fun x hx ↦ (Qs x hx).bot_not_mem
+  -- sSup_eq' := by
+  --   simp_rw [sSup_iUnion, Partition.sSup_eq, ← P.sSup_eq, sSup_eq_iSup, iSup_subtype]; rfl
+
+-- @[simp] lemma mem_bind_iff {P : Partition s} {Qs : ∀ a ∈ P, Partition a} {a : α} :
+--     a ∈ P.bind Qs ↔ ∃ (b : α) (hb : b ∈ P), a ∈ Qs b hb := by
+--   change _ ∈ ⋃ _, _ ↔ _; simp
+
+-- @[simp] lemma bind_le {α : Type*} [CompleteDistribLattice α] {s : α} (P : Partition s)
+--     (Qs : ∀ a ∈ P, Partition a) : P.bind Qs ≤ P := by
+--   intro t ht
+--   obtain ⟨b, hbp, h⟩ := mem_bind_iff.1 ht
+--   exact ⟨b, hbp, Partition.le_of_mem _ h⟩
+
+end Bind
+
+section Set
+
+variable {s t u : Set α} {P : Partition (Set α)} {x : α}
+
+@[simp] protected lemma sUnion_eq (P : Partition (Set α)) : ⋃₀ P = P.supp :=
+  P.sSup_eq
+
+lemma nonempty_of_mem (ht : t ∈ P) : t.Nonempty :=
+  nmem_singleton_empty.1 <| P.ne_bot_of_mem ht
+
+lemma subset_of_mem (ht : t ∈ P) : t ⊆ P.supp :=
+  P.le_of_mem ht
+
+lemma eq_of_mem_inter (ht : t ∈ P) (hu : u ∈ P) (hx : x ∈ t ∩ u) : t = u :=
+  PairwiseDisjoint.elim P.pairwiseDisjoint ht hu fun
+    (hdj : Disjoint t u) ↦ by simp [hdj.inter_eq] at hx
+
+lemma eq_of_mem_of_mem (ht : t ∈ P) (hu : u ∈ P) (hxt : x ∈ t) (hxu : x ∈ u) : t = u :=
+  eq_of_mem_inter ht hu ⟨hxt, hxu⟩
+
+lemma exists_unique_of_mem_set (P : Partition (Set α)) (hx : x ∈ P.supp) : ∃! t, t ∈ P ∧ x ∈ t := by
+  rw [← P.sUnion_eq, mem_sUnion] at hx
+  obtain ⟨t, hxt⟩ := hx
+  exact ⟨t, hxt, fun u ⟨huP, hxu⟩ ↦ eq_of_mem_inter huP hxt.1 ⟨hxu, hxt.2⟩⟩
+
+/-- The part containing a given element of the set being partitioned. If `x ∉ s`, then `∅`.  -/
+def partOf (P : Partition (Set α)) (x : α) : Set α :=
+  ⋃₀ {t ∈ P | x ∈ t}
+
+lemma partOf_mem (P : Partition (Set α)) (hx : x ∈ P.supp) : P.partOf x ∈ P := by
+  obtain ⟨t, ⟨h', h⟩⟩ := P.exists_unique_of_mem_set hx
+  have hrw : {t | t ∈ P ∧ x ∈ t} = {t} := by
+    ext t'
+    simp only [mem_setOf_eq, mem_singleton_iff]
+    exact ⟨h t', by rintro rfl; exact h'⟩
+  rw [partOf, hrw, sUnion_singleton]
+  exact h'.1
+
+lemma partOf_eq_empty (P : Partition (Set α)) (hx : x ∉ P.supp) : P.partOf x = ∅ := by
+  rw [← P.sUnion_eq] at hx
+  simp only [partOf, eq_empty_iff_forall_not_mem, mem_sUnion, mem_setOf, not_exists, not_and,
+    and_imp]
+  exact fun y t ht hxt _ ↦ hx <| mem_sUnion_of_mem hxt ht
+
+lemma mem_partOf (P : Partition (Set α)) (hx : x ∈ P.supp) : x ∈ P.partOf x := by
+  obtain ⟨_, ⟨h, -⟩⟩ := P.exists_unique_of_mem_set hx
+  exact mem_sUnion_of_mem h.2 h
+
+lemma eq_partOf_of_mem {P : Partition (Set α)} (ht : t ∈ P) (hxt : x ∈ t) :
+    t = P.partOf x := by
+  have hx : x ∈ P.supp := by
+    rw [← P.sUnion_eq]
+    exact mem_sUnion_of_mem hxt ht
+  obtain ⟨t', ⟨-, h⟩⟩ := P.exists_unique_of_mem_set hx
+  rw [h t ⟨ht, hxt⟩, h (P.partOf x) ⟨P.partOf_mem hx, P.mem_partOf hx⟩]
+
+/-- Noncomputably choose a representative from an equivalence class-/
+noncomputable def rep (P : Partition (Set α)) (ht : t ∈ P) : α := (P.nonempty_of_mem ht).some
+
+@[simp] lemma rep_mem (ht : t ∈ P) : P.rep ht ∈ t :=
+  (P.nonempty_of_mem ht).some_mem
+
+@[simp] lemma rep_mem' (ht : t ∈ P) : P.rep ht ∈ P.supp :=
+  P.subset_of_mem ht <| rep_mem ht
+
+@[simp] lemma partOf_rep (ht : t ∈ P) : P.partOf (P.rep ht) = t :=
+  (eq_partOf_of_mem ht (P.rep_mem ht)).symm
+
+lemma finite_of_finite (P : Partition (Set α)) (hs : P.supp.Finite) : (P : Set (Set α)).Finite :=
+  hs.finite_subsets.subset fun _ ↦ subset_of_mem
+
+@[simps] def ofPairwiseDisjoint {p : Set (Set α)} (h : p.PairwiseDisjoint id) (h_empty : ∅ ∉ p):
+    Partition (Set α) where
+  parts := p
+  indep := PairwiseDisjoint.sSupIndep h
+  bot_not_mem := h_empty
+
+lemma ofPairwiseDisjoint_supp {p : Set (Set α)} (h : p.PairwiseDisjoint id) (h_empty : ∅ ∉ p) :
+    (ofPairwiseDisjoint h h_empty).supp = ⋃₀ p := rfl
+
+end Set
+
 section Rel
 
-variable {s t : Set α} {a b : α} {P : Partition s}
+variable {s t : Set α} {a b : α} {P : Partition (Set α)}
+
+lemma symm_iff_of {α : Type*} (r : α → α → Prop) [IsSymm α r] {x y : α} : r x y ↔ r y x :=
+  ⟨fun h ↦ symm_of r h, fun h ↦ symm_of r h⟩
+
+lemma refl_of_rel {α : Type*} (r : α → α → Prop) [IsSymm α r] [IsTrans α r] {x y : α}
+    (h : r x y) : r x x :=
+  trans_of r h (symm_of r h)
+
+/-- A transitive, symmetric Binary relation `r` induces a partition of the set of elements on
+  which it is reflexive. -/
+@[simps] def ofRel (r : α → α → Prop) [IsTrans α r] [IsSymm α r] : Partition (Set α) where
+  parts := ((fun a ↦ {x | r a x}) '' {x | r x x})
+  indep := by
+    apply PairwiseDisjoint.sSupIndep
+    rintro _ ⟨i, -, rfl⟩ _ ⟨j, -,rfl⟩ hij
+    refine disjoint_iff_forall_ne.2 ?_
+    rintro a (ha : r _ _) _ (hb : r _ _) rfl
+    simp only [ne_eq, Set.ext_iff, mem_setOf_eq, not_forall] at hij
+    obtain ⟨y, hy⟩ := hij
+    exact hy ⟨fun hiy ↦ trans_of r hb (trans_of r (symm_of r ha) hiy),
+      fun hjy ↦ trans_of r ha (trans_of r (symm_of r hb) hjy)⟩
+  bot_not_mem := by
+    simp only [bot_eq_empty, mem_image, mem_setOf_eq, eq_empty_iff_forall_not_mem, not_exists,
+      not_and, not_forall, not_not]
+    exact fun x hx ↦ ⟨x,hx⟩
 
 @[simp]
-lemma rel_ofRel'_eq (r : α → α → Prop) [IsTrans α r] [IsSymm α r] (hs : s = {x | r x x}) :
-    (ofRel' r hs).Rel = r := by
-  simp only [ofRel', rel_congr, rel_ofRel_eq]
+lemma ofRel_supp {r : α → α → Prop} [IsTrans α r] [IsSymm α r] : (ofRel r).supp = {x | r x x} := by
+  rw [supp, ofRel, sSup_eq_sUnion, subset_antisymm_iff]
+  simp only [sUnion_image, mem_setOf_eq, iUnion_subset_iff, setOf_subset_setOf]
+  refine ⟨fun i _ a ha ↦ trans_of r (symm_of r ha) ha, fun i (hi : r i i) ↦ ?_⟩
+  simp only [mem_iUnion, mem_setOf_eq, exists_prop]
+  exact ⟨i, hi, hi⟩
+
+variable {r : α → α → Prop} [IsSymm α r] [IsTrans α r] {s : Set α}
+
+lemma eqv_class_comm {r : α → α → Prop} [IsSymm α r] (x : α) : {y | r x y} = {y | r y x} := by
+  simp_rw [symm_iff_of]
+
+lemma rel_iff_eqv_class_eq_right (hy : r y y) : r x y ↔ {z | r x z} = {z | r y z} := by
+  simp_rw [Set.ext_iff, mem_setOf]
+  exact ⟨fun hxy z ↦ ⟨fun hxz ↦ trans_of r (symm_of r hxy) hxz,
+    fun hyz ↦ trans_of r hxy hyz⟩, fun h ↦ by rwa [h]⟩
+
+lemma rel_iff_eqv_class_eq_left (hx : r x x) : r x y ↔ {z | r x z} = {z | r y z} := by
+  rw [symm_iff_of r, rel_iff_eqv_class_eq_right hx, eq_comm]
+
+lemma eqv_class_mem_ofRel (h : r x x) : {y | r x y} ∈ ofRel r :=
+  ⟨x, h, rfl⟩
+
+@[simp] lemma mem_ofRel_iff {t : Set α} :
+    t ∈ ofRel r ↔ ∃ x, r x x ∧ t = {y | r x y} := by
+  simp_rw [eq_comm (a := t)]; rfl
+
+lemma class_nonempty {t : Set α} (ht : t ∈ ofRel r) : t.Nonempty := by
+  obtain ⟨x, hx, rfl⟩ := ht; exact ⟨x, hx⟩
+
+/-- Every partition of `s : Set α` induces a transitive, symmetric Binary relation on `α`
+  whose equivalence classes are the parts of `P`. The relation is irreflexive outside `s`.  -/
+def Rel (P : Partition (Set α)) (a b : α) : Prop :=
+  ∃ t ∈ P, a ∈ t ∧ b ∈ t
+
+lemma Rel.exists (h : P.Rel x y) : ∃ t ∈ P, x ∈ t ∧ y ∈ t :=
+  h
+
+lemma Rel.forall (h : P.Rel x y) (ht : t ∈ P) : x ∈ t ↔ y ∈ t := by
+  obtain ⟨t', ht', hx, hy⟩ := h
+  exact ⟨fun h ↦ by rwa [P.eq_of_mem_of_mem ht ht' h hx],
+    fun h ↦ by rwa [P.eq_of_mem_of_mem ht ht' h hy]⟩
+
+lemma rel_of_mem_of_mem (ht : t ∈ P) (ha : a ∈ t) (hb : b ∈ t) : P.Rel a b :=
+  ⟨t, ht, ha, hb⟩
+
+lemma rel_self_of_mem (ht : t ∈ P) (hx : x ∈ t) : P.Rel x x :=
+  rel_of_mem_of_mem ht hx hx
+
+instance (P : Partition (Set α)) : IsSymm α P.Rel where
+  symm _ _ := fun ⟨t, ht, ha, hb⟩ ↦ ⟨t, ht, hb, ha⟩
+
+instance (P : Partition (Set α)) : IsTrans α P.Rel where
+  trans a b c := fun ⟨t, htP, ha, hb⟩ ⟨t', ht'P, hb', hc'⟩ ↦
+    ⟨t, htP, ha, by rwa [eq_of_mem_of_mem htP ht'P hb hb']⟩
+
+lemma Rel.symm {P : Partition (Set α)} (h : P.Rel x y) : P.Rel y x :=
+  symm_of P.Rel h
+
+lemma rel_comm {P : Partition (Set α)} : P.Rel x y ↔ P.Rel y x :=
+  ⟨Rel.symm, Rel.symm⟩
+
+lemma Rel.trans {P : Partition (Set α)} (hxy : P.Rel x y) (hyz : P.Rel y z) : P.Rel x z :=
+  trans_of P.Rel hxy hyz
+
+lemma Rel.mem_left {P : Partition (Set α)} (h : P.Rel x y) : x ∈ P.supp := by
+  obtain ⟨t, htP, hxt, -⟩ := h
+  exact subset_of_mem htP hxt
+
+lemma Rel.mem_right {P : Partition (Set α)} (h : P.Rel x y) : y ∈ P.supp :=
+  h.symm.mem_left
+
+lemma rel_iff_exists : P.Rel x y ↔ ∃ t ∈ P, x ∈ t ∧ y ∈ t := Iff.rfl
+
+lemma rel_iff_partOf_eq_partOf (P : Partition (Set α)) (hx : x ∈ P.supp) (hy : y ∈ P.supp) :
+    P.Rel x y ↔ P.partOf x = P.partOf y := by
+  refine ⟨fun ⟨t, htP, hxt, hyt⟩ ↦ ?_, fun h ↦ ⟨P.partOf x, P.partOf_mem hx, P.mem_partOf hx, ?_⟩⟩
+  · rw [eq_partOf_of_mem (P.partOf_mem hx)]
+    rwa [← eq_partOf_of_mem htP hxt]
+  rw [h]
+  exact mem_partOf P hy
+
+lemma rel_iff_partOf_eq_partOf' (P : Partition (Set α)) :
+    P.Rel x y ↔ ∃ (_ : x ∈ P.supp) (_ : y ∈ P.supp), P.partOf x = P.partOf y :=
+  ⟨fun h ↦ ⟨h.mem_left, h.mem_right, (P.rel_iff_partOf_eq_partOf h.mem_left h.mem_right).1 h⟩,
+    fun ⟨hx,hy,h⟩ ↦ (P.rel_iff_partOf_eq_partOf hx hy).2 h⟩
+
+lemma rel_iff_forall {P : Partition (Set α)} : P.Rel x y ↔ x ∈ P.supp ∧ ∀ t ∈ P, x ∈ t ↔ y ∈ t := by
+  refine ⟨fun h ↦ ⟨h.mem_left, fun _ ↦ h.forall⟩,
+    fun ⟨hxs, h⟩ ↦ ⟨P.partOf x, P.partOf_mem hxs, P.mem_partOf hxs, ?_⟩⟩
+  rw [← h _ (P.partOf_mem hxs)]
+  exact P.mem_partOf hxs
+
+lemma setOf_rel_self_eq (P : Partition (Set α)) : {x | P.Rel x x} = P.supp := by
+  refine subset_antisymm (fun x hx ↦ ?_) (fun x hx ↦ ?_)
+  · obtain ⟨t, ht, hxP, -⟩ := hx
+    exact subset_of_mem ht hxP
+  obtain ⟨t, ⟨ht, hxt⟩, -⟩ := P.exists_unique_of_mem_set hx
+  exact ⟨t, ht, hxt, hxt⟩
+
+lemma rel_self_iff_mem {P : Partition (Set α)} : P.Rel x x ↔ x ∈ P.supp := by
+  simp [← P.setOf_rel_self_eq]
+
+lemma setOf_rel_eq (ht : t ∈ P) (hx : x ∈ t) : {y | P.Rel x y} = t :=
+  Set.ext fun y ↦ ⟨fun ⟨t', ht', hx', hy'⟩ ↦ by rwa [P.eq_of_mem_of_mem ht ht' hx hx'],
+    fun h ↦ ⟨t, ht, hx, h⟩⟩
+
+lemma rep_rel (ht : t ∈ P) (hx : x ∈ t) : P.Rel x (P.rep ht) :=
+  ⟨t, ht, hx, P.rep_mem ht⟩
+
+@[simp] lemma rep_rel_self {P : Partition (Set α)} (ht : t ∈ P) : P.Rel (P.rep ht) (P.rep ht) :=
+  rep_rel _ (P.rep_mem ht)
+
+lemma setOf_rel_rep_eq (ht : t ∈ P) : {x | P.Rel (P.rep ht) x} = t :=
+  setOf_rel_eq ht (P.rep_mem ht)
+
+/-- The `partOf x` is the set of `y` related to `x`. True even if `x ∉ s`, since both are `∅`.-/
+lemma setOf_rel_eq_partOf (P : Partition (Set α)) (x : α) : {y | P.Rel x y} = P.partOf x := by
+  by_cases hx : x ∈ P.supp
+  · rw [setOf_rel_eq (P.partOf_mem hx) (P.mem_partOf hx)]
+  rw [partOf_eq_empty _ hx, eq_empty_iff_forall_not_mem]
+  exact fun y hxy ↦ hx <| Rel.mem_left hxy
+
+lemma setOf_rel_mem (P : Partition (Set α)) (hx : x ∈ P.supp) : {y | P.Rel x y} ∈ P := by
+  obtain ⟨t, ⟨ht,hp⟩, -⟩ := P.exists_unique_of_mem_set hx
+  rwa [setOf_rel_eq ht hp]
+
+lemma ofRel_rel_eq (P : Partition (Set α)) : ofRel P.Rel = P := by
+  ext a
+  simp only [mem_ofRel_iff]
+  refine ⟨?_, fun h ↦ ?_⟩
+  · rintro ⟨x, hx, rfl⟩
+    exact setOf_rel_mem _ hx.mem_right
+  obtain ⟨x, hx⟩ := P.nonempty_of_mem h
+  exact ⟨x, rel_of_mem_of_mem h hx hx, by rwa [setOf_rel_eq _ hx]⟩
+
+@[simp] lemma rel_ofRel_eq (r : α → α → Prop) [IsTrans α r] [IsSymm α r] : (ofRel r).Rel = r := by
+  ext a b
+  simp only [Rel, mem_ofRel_iff]
+  refine ⟨?_, fun h ↦ ⟨_, ⟨a, refl_of_rel r h, rfl⟩, refl_of_rel r h, h⟩⟩
+  rintro ⟨_, ⟨x, -, rfl⟩, ha, hb⟩
+  exact trans_of r (symm_of r ha) hb
+
+@[ext] theorem eq_of_rel_iff_rel {P P' : Partition (Set α)} (h : ∀ x y, P.Rel x y ↔ P'.Rel x y) :
+    P = P' := by
+  rw [← ofRel_rel_eq P, ← ofRel_rel_eq P']; congr; ext; exact h _ _
 
 end Rel
+
+section Discrete
+
+variable {s : Set α} {a b : α}
+
+/-- The discrete partition -/
+protected def discrete (s : Set α) : Partition (Set α) :=
+  let r : α → α → Prop := fun x y ↦ x = y ∧ x ∈ s
+  have : IsTrans α r := ⟨by rintro _ _ _ ⟨rfl, h⟩ ⟨rfl,-⟩; exact ⟨rfl, h⟩⟩
+  have : IsSymm α r := ⟨by rintro _ _ ⟨rfl, h⟩; exact ⟨rfl,h⟩⟩
+  ofRel r
+
+@[simp] lemma discrete.supp : (Partition.discrete s).supp = s := by
+  simp [Partition.discrete]
+
+@[simp] lemma discrete.rel_iff_eq : (Partition.discrete s).Rel a b ↔ a = b ∧ a ∈ s := by
+  simp only [Partition.discrete, rel_ofRel_eq]
+
+lemma discrete.rel_iff_eq_of_mem (ha : a ∈ s) : (Partition.discrete s).Rel a b ↔ a = b := by
+  rw [discrete.rel_iff_eq, and_iff_left ha]
+
+end Discrete
+
+section RepFun
+
+variable {a b : α} {P : Partition (Set α)}
+
+structure RepFun (P : Partition (Set α)) where
+  (toFun : α → α)
+  (apply_eq_self_of_not_mem : ∀ a ∉ P.supp, toFun a = a)
+  (rel_apply_of_mem : ∀ a ∈ P.supp, P.Rel a (toFun a))
+  (apply_eq_of_rel : ∀ a b, P.Rel a b → toFun a = toFun b)
+
+instance : FunLike (RepFun P) α α where
+  coe := RepFun.toFun
+  coe_injective' f f' := by cases f; cases f'; simp
+
+@[simp] lemma RepFun.mk_apply (P : Partition (Set α)) (f) (h₁ : ∀ a ∉ P.supp, f a = a)
+  (h₂ : ∀ a ∈ P.supp, P.Rel a (f a)) (h₃) (x : α) : (RepFun.mk f h₁ h₂ h₃) x = f x := rfl
+
+lemma RepFun.apply_of_not_mem (f : P.RepFun) (ha : a ∉ P.supp) : f a = a :=
+  f.apply_eq_self_of_not_mem a ha
+
+lemma RepFun.rel_apply (f : P.RepFun) (ha : a ∈ P.supp) : P.Rel a (f a) :=
+  f.rel_apply_of_mem a ha
+
+lemma RepFun.apply_mem (f : P.RepFun) (ha : a ∈ P.supp) : f a ∈ P.supp :=
+  (f.rel_apply ha).mem_right
+
+lemma RepFun.apply_eq_apply (f : P.RepFun) (hab : P.Rel a b) : f a = f b :=
+  f.apply_eq_of_rel a b hab
+
+lemma RepFun.rel_of_apply_eq_apply (f : P.RepFun) (ha : a ∈ P.supp) (hab : f a = f b) : P.Rel a b := by
+  refine (f.rel_apply ha).trans ?_
+  rw [hab, P.rel_comm]
+  refine f.rel_apply <| by_contra fun hb ↦ ?_
+  rw [f.apply_of_not_mem hb] at hab; rw [← hab] at hb
+  exact hb <| f.apply_mem ha
+
+lemma RepFun.rel_of_ne_of_apply_eq_apply (f : P.RepFun) (hne : a ≠ b) (hab : f a = f b) :
+    P.Rel a b := by
+  obtain (ha | ha) := em (a ∈ P.supp); exact f.rel_of_apply_eq_apply ha hab
+  obtain (hb | hb) := em (b ∈ P.supp); exact (f.rel_of_apply_eq_apply hb hab.symm).symm
+  rw [f.apply_of_not_mem ha, f.apply_of_not_mem hb] at hab; contradiction
+
+lemma RepFun.apply_eq_apply_iff_rel (f : P.RepFun) (ha : a ∈ P.supp) : f a = f b ↔ P.Rel a b :=
+  ⟨f.rel_of_apply_eq_apply ha, f.apply_eq_apply⟩
+
+lemma RepFun.apply_eq_apply_iff_rel_of_ne (f : P.RepFun) (hne : a ≠ b) : f a = f b ↔ P.Rel a b :=
+  ⟨f.rel_of_ne_of_apply_eq_apply hne, f.apply_eq_apply⟩
+
+@[simp] lemma RepFun.idem (f : P.RepFun) (a : α) : f (f a) = f a := by
+  obtain (ha | ha) := em (a ∈ P.supp)
+  · rw [eq_comm, f.apply_eq_apply_iff_rel ha]
+    exact f.rel_apply ha
+  simp_rw [f.apply_of_not_mem ha]
+
+lemma RepFun.image_subset_self (f : P.RepFun) : f '' P.supp ⊆ P.supp := by
+  rintro _ ⟨a,ha,rfl⟩; exact f.apply_mem ha
+
+/-- Any partially defined `RepFun` extends to a complete one. -/
+lemma exists_extend_partial_repFun (P : Partition (Set α)) {t : Set α} (f₀ : t → α)
+    (h_not_mem : ∀ x : t, x.1 ∉ P.supp → f₀ x = x) (h_mem : ∀ x : t, x.1 ∈ P.supp → P.Rel x (f₀ x))
+    (h_eq : ∀ x y : t, P.Rel x y → f₀ x = f₀ y) : ∃ (f : P.RepFun), ∀ x : t, f x = f₀ x := by
+  classical
+  set f : α → α := fun a ↦ if ha : a ∈ P.supp then
+    (if hb : ∃ b : t, P.Rel a b then f₀ hb.choose else P.rep (P.partOf_mem ha)) else a with hf
+  refine ⟨RepFun.mk f (fun a ha ↦ by simp [hf, ha]) (fun a ha ↦ ?_) (fun a b hab ↦ ?_), fun a ↦ ?_⟩
+  · simp only [hf, exists_prop, ha, ↓reduceDIte]
+    split_ifs with h
+    · exact h.choose_spec.trans <| h_mem h.choose h.choose_spec.mem_right
+    push_neg at h
+    exact P.rep_rel (P.partOf_mem ha) (P.mem_partOf ha)
+  · simp_rw [hf, dif_pos hab.mem_left, dif_pos hab.mem_right]
+    split_ifs with h₁ h₂ h₂
+    · exact h_eq _ _ <| (hab.symm.trans h₁.choose_spec).symm.trans h₂.choose_spec
+    · exact False.elim <| h₂ ⟨_, hab.symm.trans h₁.choose_spec⟩
+    · exact False.elim <| h₁ ⟨_, hab.trans h₂.choose_spec⟩
+    congr
+    rwa [← rel_iff_partOf_eq_partOf _ hab.mem_left hab.mem_right]
+  change f a = f₀ a
+  obtain (ha | ha) := em (a.1 ∈ P.supp)
+  · simp only [hf, exists_prop, ha, ↓reduceDIte]
+    split_ifs with h
+    · exact Eq.symm <| h_eq _ _ h.choose_spec
+    exact False.elim <| h ⟨a, rel_self_iff_mem.2 ha⟩
+  simp [hf, ha, h_not_mem _ ha]
+
+/-- For any set `t` containining no two distinct related elements, there is a `RepFun` equal to
+the identity on `t`. -/
+lemma exists_extend_partial_repFun' (P : Partition (Set α)) {t : Set α}
+    (h : ∀ ⦃x y⦄, x ∈ t → y ∈ t → P.Rel x y → x = y) : ∃ (f : P.RepFun), EqOn f id t := by
+  simpa using P.exists_extend_partial_repFun (fun x : t ↦ x) (by simp)
+    (by simp [P.rel_self_iff_mem]) (fun x y ↦ h x.2 y.2)
+
+lemma nonempty_repFun (P : Partition (Set α)) : Nonempty P.RepFun := by
+  obtain ⟨f, -⟩ := P.exists_extend_partial_repFun' (t := ∅) (by simp)
+  exact ⟨f⟩
+
+@[simp] theorem repFun_repFun (f f' : P.RepFun) (x : α) : f (f' x) = f x := by
+  obtain (hx | hx) := em (x ∈ P.supp)
+  · exact f.apply_eq_apply (f'.rel_apply hx).symm
+  rw [f'.apply_of_not_mem hx, f.apply_of_not_mem hx]
+
+@[simp] lemma repFun_discrete_coeFun (s : Set α) (f : (Partition.discrete s).RepFun) :
+    (f : α → α) = id := by
+  ext x
+  obtain (hx | hx) := em (x ∈ s)
+  · have hx' := f.rel_apply (by simpa)
+    simp only [discrete.rel_iff_eq] at hx'
+    exact hx'.1.symm
+  rw [f.apply_of_not_mem (by simpa), id]
+
+lemma RepFun.coeFun_eq_id_of_eq_discrete {s : Set α} (f : P.RepFun) (hP : P = Partition.discrete s) :
+    (f : α → α) = id := by
+  subst hP; exact repFun_discrete_coeFun s f
+
+end RepFun
